impl to low for point funcs

src/zksync_verifier.ec
@@ -1,6 +1,7 @@
 pragma Goals:printall.
 
 require import Array.
+require import EllipticCurve.
 require import Logic.
 require import Memory.
 require import PurePrimops.
@@ -10,9 +11,11 @@ require import Utils.
 require import YulPrimops.
 require import Verifier.
 
+import MemoryMap.
+
 op p_int = 21888242871839275222246405745257275088696311157297823662689037894645226208583.
 op p_uint256 = W256.of_int p_int.
-  
+
 (* Functional correctness *)
 
 lemma usr_revertWithMessage_correctness :
@@ -43,7 +46,7 @@ module PointNegate = {
     if (y <> W256.zero) {
         Primops.mstore(point + W256.of_int 32, p_uint256 - y);
     }
-    
+
     if (x <> W256.zero /\ y = W256.zero) {
       Primops.revert(W256.zero, W256.zero);
     }
@@ -121,15 +124,15 @@ lemma pointNegate_actual_matches_low: equiv [
       skip. by progress.
       progress.                                                                    (* to prove: x loaded correct in actual *)
       wp.
-      call (ConcretePrimops.mload_spec memory point).   
+      call (ConcretePrimops.mload_spec memory point).
       inline Primops.mload. wp. skip. by progress.
       progress.                                                                  (* to prove: y loaded correctly in low *)
       call (ConcretePrimops.mload_spec memory (point + W256.of_int 32)).
       inline Primops.mload. wp. skip. by progress.
       progress.                                                                  (* to prove: y loaded correctly in actual *)
-      wp.                                                                         
-      call (ConcretePrimops.mload_spec memory (point + W256.of_int 32)).         
-      wp. skip. by progress.                                                     
+      wp.
+      call (ConcretePrimops.mload_spec memory (point + W256.of_int 32)).
+      wp. skip. by progress.
                                                                              (* case y<>0 *)
       rcondf{1} 6; first last.                                                 (* actual: take writing branch *)
       rcondf{2} 4; first last.                                                 (* low: skip reverting branch *)
@@ -151,8 +154,8 @@ lemma pointNegate_actual_matches_low: equiv [
       call (ConcretePrimops.mload_spec memory (point + W256.of_int 32)).
       wp. skip. by progress.
   qed.
-    
-lemma pointNegate_low_matches_mid (memory: mem) (point_address: uint256) (point_x_int point_y_int: int): equiv [
+
+lemma pointNegate_low_matches_mid (memory: MemoryMap.mem) (point_address: uint256) (point_x_int point_y_int: int): equiv [
     PointNegate.low ~ PointNegate.mid :
       arg{2} = (point_x_int, point_y_int) /\
       arg{1} = point_address /\
@@ -216,7 +219,7 @@ lemma pointNegate_low_matches_mid (memory: mem) (point_address: uint256) (point_
       call{1} (ConcretePrimops.mload_pspec memory_pre point_address).
       wp. skip. by progress.
     qed.
-    
+
 lemma pointNegate_mid_matches_high (point: Point):
   equiv [
     PointNegate.mid ~ PointNegate.high :
@@ -232,3 +235,222 @@ lemma pointNegate_mid_matches_high (point: Point):
     proc.
     wp. skip. progress; by smt().
 qed.
+
+module PointAddAssign = {
+  proc low(usr_p1, usr_p2) =
+  {
+    var _1, _5, _6, _9, _13, _14, tmp78;
+    _1 <@ Primops.mload(usr_p1);
+    Primops.mstore(W256.zero, _1);
+    _5 <@ Primops.mload(usr_p1 + W256.of_int 32);
+    Primops.mstore(W256.of_int 32, _5);
+    _6 <@ Primops.mload(usr_p2);
+    Primops.mstore(W256.of_int 64, _6);
+    _9 <@ Primops.mload(usr_p2 + W256.of_int 32);
+    Primops.mstore(W256.of_int 96, _9);
+    _13 <@ Primops.gas();
+    _14 <@ Primops.staticcall(_13, W256.of_int 6, W256.zero, W256.of_int 128, usr_p1, W256.of_int 64);
+    if ((bool_of_uint256 (PurePrimops.iszero _14)))
+      {
+      tmp78 <@ Verifier.usr_revertWithMessage(W256.of_int 28, (W256.of_int STRING (*pointAddAssign: ecAdd failed*)));
+      }
+  }
+}.
+
+lemma usr_pointAddAssign_actual_matches_low (x y : uint256) : equiv [
+    Verifier.usr_pointAddAssign ~ PointAddAssign.low :
+      ={Primops.memory} /\
+      ={arg} /\
+      ={Primops.reverted} /\
+      !Primops.reverted{1}
+      ==>
+        (Primops.reverted{1} <=> Primops.reverted{2}) /\
+        (!Primops.reverted{1}) =>
+        forall (idx: uint256),
+        Primops.memory{1}.[idx] =
+        Primops.memory{2}.[idx]
+    ].
+proof.
+  proc.  
+  seq 24 10: (#pre /\ ={_1, _5, _6, _9, _13, _14} /\ _2{1} = W256.zero /\ _3{1} = W256.of_int 32 /\ _4{1} = usr_p1{1} + _3{1}
+             /\ _7{1} = W256.of_int 64 /\ _8{1} = usr_p2{1} + _3{1} /\ _10{1} = W256.of_int 96 /\ _11{1} = W256.of_int 128
+             /\ _12{1} = W256.of_int 6).
+  inline*. wp. skip. progress.
+  inline*. wp. skip. progress.
+qed. 
+
+module PointAddIntoDest = {
+  proc low(usr_p1, usr_p2, usr_dest) =
+  {
+    var _1, _5, _6, _9, _13, _14, tmp64;
+    _1 <@ Primops.mload(usr_p1);
+    Primops.mstore(W256.of_int 0, _1);
+    _5 <@ Primops.mload(usr_p1 + W256.of_int 32);
+    Primops.mstore(W256.of_int 32, _5);
+    _6 <@ Primops.mload(usr_p2);
+    Primops.mstore(W256.of_int 64, _6);
+    _9 <@ Primops.mload(usr_p2 + W256.of_int 32);
+    Primops.mstore(W256.of_int 96, _9);
+    _13 <@ Primops.gas();
+    _14 <@ Primops.staticcall(_13, W256.of_int 6, W256.zero, W256.of_int 128, usr_dest, W256.of_int 64);
+    if ((bool_of_uint256 (PurePrimops.iszero _14)))
+      {
+      tmp64 <@ Verifier.usr_revertWithMessage((W256.of_int 30), (W256.of_int STRING (*pointAddIntoDest: ecAdd failed*)));
+      }
+  }
+}.
+
+lemma usr_pointAddIntoDest_actual_matches_low (x y : uint256) : equiv [
+    Verifier.usr_pointAddIntoDest ~ PointAddIntoDest.low :
+      ={Primops.memory} /\
+      ={arg} /\
+      ={Primops.reverted} /\
+      !Primops.reverted{1}
+      ==>
+        (Primops.reverted{1} <=> Primops.reverted{2}) /\
+        (!Primops.reverted{1}) =>
+        forall (idx: uint256),
+        Primops.memory{1}.[idx] =
+        Primops.memory{2}.[idx]
+    ].
+proof.
+  proc.
+  seq 24 10: (#pre /\ ={_1, _5, _6, _9, _13, _14} /\ _2{1} = W256.zero /\ _3{1} = W256.of_int 32 /\ _4{1} = usr_p1{1} + _3{1}
+             /\ _7{1} = W256.of_int 64 /\ _8{1} = usr_p2{1} + _3{1} /\ _10{1} = W256.of_int 96 /\ _11{1} = W256.of_int 128
+             /\ _12{1} = W256.of_int 6).
+  inline*. wp. skip. progress.
+  inline*. wp. skip. progress.
+qed.
+
+module PointMulIntoDest = {
+  proc low(usr_point, usr_s, usr_dest) =
+  {
+    var _1, _5,  _9, _10;
+    _1 <@ Primops.mload(usr_point);
+    Primops.mstore(W256.zero, _1);
+    _5 <@ Primops.mload(usr_point + W256.of_int 32);
+    Primops.mstore(W256.of_int 32, _5);
+    Primops.mstore(W256.of_int 64, usr_s);
+    _9 <@ Primops.gas();
+    _10 <@ Primops.staticcall(_9, W256.of_int 7, W256.zero, W256.of_int 96, usr_dest, W256.of_int 64);
+    if (bool_of_uint256 (PurePrimops.iszero(_10)))
+    {
+      Verifier.usr_revertWithMessage(W256.of_int 30, W256.zero);
+    }
+  }
+}.
+
+lemma usr_pointMulIntoDest_actual_matches_low (x y : uint256) : equiv [
+    Verifier.usr_pointMulIntoDest ~ PointMulIntoDest.low :
+      ={Primops.memory} /\
+      ={arg} /\
+      ={Primops.reverted} /\
+      !Primops.reverted{1}
+      ==>
+        (Primops.reverted{1} <=> Primops.reverted{2}) /\
+        (!Primops.reverted{1}) =>
+        forall (idx: uint256),
+        Primops.memory{1}.[idx] =
+        Primops.memory{2}.[idx]
+    ].
+proof.
+  proc.
+  seq 17 7: (#pre /\ ={_1} /\ _2{1} = W256.zero /\ _3{1} = W256.of_int 32 /\ _4{1} = usr_point{1} + _3{1}
+            /\ _6{1} = W256.of_int 64 /\ _7{1} = W256.of_int 96 /\ _8{1} = W256.of_int 7 /\ ={_5, _9, _10}).
+  inline*. wp. skip. progress.
+  inline*. wp. skip. progress.
+qed.
+
+module PointMulAndAddIntoDest = {
+  proc low(usr_point, usr_s, usr_dest) =
+  {
+    var _1, _5, _9, usr_success, _10, _12, _15, _16, tmp87;
+    _1 <@ Primops.mload(usr_point);
+    Primops.mstore(W256.zero, _1);
+    _5 <@ Primops.mload(usr_point + W256.of_int 32);
+    Primops.mstore(W256.of_int 32, _5);
+    Primops.mstore(W256.of_int 64, usr_s);
+    _9 <@ Primops.gas();
+    usr_success <@ Primops.staticcall(_9, W256.of_int 7, W256.zero, W256.of_int 96, W256.zero, W256.of_int 64);
+    _10 <@ Primops.mload(usr_dest);
+    Primops.mstore(W256.of_int 64, _10);
+    _12 <@ Primops.mload(usr_dest + W256.of_int 32);
+    Primops.mstore(W256.of_int 96, _12);
+    _15 <@ Primops.gas();
+    _16 <@ Primops.staticcall(_15, W256.of_int 6, W256.zero, W256.of_int 128, usr_dest, W256.of_int 64);
+    usr_success <- (PurePrimops.bit_and usr_success _16);
+    if ((bool_of_uint256 (PurePrimops.iszero usr_success)))
+      {
+      tmp87 <@ Verifier.usr_revertWithMessage(W256.of_int 22, W256.of_int STRING);
+      }
+  }
+}.
+
+lemma usr_pointMulAndAddIntoDest_actual_matches_low (x y : uint256) : equiv [
+    Verifier.usr_pointMulAndAddIntoDest ~ PointMulAndAddIntoDest.low :
+      ={Primops.memory} /\
+      ={arg} /\
+      ={Primops.reverted} /\
+      !Primops.reverted{1}
+      ==>
+        (Primops.reverted{1} <=> Primops.reverted{2}) /\
+        (!Primops.reverted{1}) =>
+        forall (idx: uint256),
+        Primops.memory{1}.[idx] =
+        Primops.memory{2}.[idx]
+    ].
+proof.
+  proc.
+  seq 20 9: (#pre /\ ={_1} /\ _2{1} = W256.zero /\ _3{1} = W256.of_int 32 /\  _4{1} = usr_point{1} + _3{1} /\
+            _6{1} = W256.of_int 64 /\ _7{1} = W256.of_int 96 /\ _8{1} = W256.of_int 7 /\ ={_5, _9, usr_success, _10}).
+  inline*. wp. skip. progress. sp.
+  seq 9 4: (#pre /\ ={_12} /\ _13{1} = W256.of_int 128 /\ _14{1} = W256.of_int 6 /\ ={_15, _16}).
+  inline*. wp. skip. progress.
+  inline*. wp. skip. progress.
+qed.
+
+
+module PointSubAssign = {
+  proc low(usr_p1, usr_p2) =
+  {
+    var _1, _5, _6, _9, _15, _16, tmp71;
+    _1 <@ Primops.mload(usr_p1);
+    Primops.mstore(W256.zero, _1);
+    _5 <@ Primops.mload(usr_p1 + W256.of_int 32);
+    Primops.mstore(W256.of_int 32, _5);
+    _6 <@ Primops.mload(usr_p2);
+    Primops.mstore(W256.of_int 64, _6);
+    _9  <@ Primops.mload(usr_p2 + W256.of_int 32);
+    Primops.mstore(W256.of_int 96, W256.of_int 21888242871839275222246405745257275088696311157297823662689037894645226208583 - _9);
+    _15 <@ Primops.gas();
+    _16 <@ Primops.staticcall(_15, W256.of_int 6, W256.zero, W256.of_int 128, usr_p1, W256.of_int 64);
+    if ((bool_of_uint256 (PurePrimops.iszero _16)))
+      {
+      tmp71 <@ Verifier.usr_revertWithMessage(W256.of_int 28, (W256.of_int STRING));
+      }
+  }
+}.
+
+lemma usr_pointSubAssign_actual_matches_low (x y : uint256) : equiv [
+    Verifier.usr_pointSubAssign ~ PointSubAssign.low :
+      ={Primops.memory} /\
+      ={arg} /\
+      ={Primops.reverted} /\
+      !Primops.reverted{1}
+      ==>
+        (Primops.reverted{1} <=> Primops.reverted{2}) /\
+        (!Primops.reverted{1}) =>
+        forall (idx: uint256),
+        Primops.memory{1}.[idx] =
+        Primops.memory{2}.[idx]
+      ].
+proof.
+  proc.
+  seq 16 7: (#pre /\ ={_1} /\ _2{1} = W256.zero /\ _3{1} = W256.of_int 32 /\ _4{1} = usr_p1{1} + _3{1}
+            /\ ={_5, _6, _9} /\ _7{1} = W256.of_int 64 /\ _8{1} = usr_p2{1} + _3{1}).
+  inline*. wp. skip. progress. sp.
+  seq 7 3: (#pre /\ _13{1} = W256.of_int 128 /\ _14{1} = W256.of_int 6 /\ ={_15, _16}).
+  inline*. wp. skip. progress.
+  inline*. wp. skip. progress.
+qed.  
+  
